Trying nat-indexed stackunroll next.

model.v
@@ -1,4 +1,5 @@
-Require Import ZArith NArith List.
+Require Import ZArith NArith List ListSet Paco.paco.
+Import ListNotations.
 Definition Name := nat.
 Notation "'dec_type' T" := (forall x y : T, {x=y}+{x<>y}) (at level 70, no associativity).
 
@@ -55,8 +56,8 @@ Proof.
 Inductive val :=
   | closure : Name -> Expr -> Env -> val
   | adelay : Addr -> val
-  | amany : list val -> val.
-Definition AbsVal := list val.
+  | amany : set val -> val.
+Definition AbsVal := set val.
 Axiom val_eq_dec : dec_type val.
 Definition absval_eq_dec : dec_type AbsVal.
   apply list_eq_dec,val_eq_dec.
@@ -81,17 +82,29 @@ Definition kont_eq_dec : dec_type Kont.
   apply list_eq_dec,frame_eq_dec.
 Defined.
 
-Inductive CESK :=
-  | ev : Expr -> Env -> Store -> Kont -> Time -> CESK
-  | co : val -> Store -> Kont -> Time -> CESK
+Inductive Shell (P : Type) :=
+  shell : P -> Kont -> Time -> Shell P.
+
+Inductive CES_point :=
+  | ev : Expr -> Env -> Store -> CES_point
+  | co : val -> Store -> CES_point
   | ap : Name -> Expr -> Env -> (* Closure *)
          val -> (* Argument *)
-         Store -> Kont -> Time -> CESK.
+         Store -> CES_point.
+Definition CESK := Shell CES_point.
 
-Definition cesk_eq_dec : dec_type CESK.
+Definition ces_point_eq_dec : dec_type CES_point.
   decide equality; try solve [apply expr_eq_dec | apply env_eq_dec | apply kont_eq_dec
                              | apply time_eq_dec | apply val_eq_dec | apply store_eq_dec | apply name_eq_dec].
 Defined.
+
+Definition cesk_eq_dec : dec_type CESK.
+  decide equality; try solve [apply kont_eq_dec | apply time_eq_dec | apply ces_point_eq_dec].
+Defined.
+
+Inductive InDom {A B} : list (A * B) -> A -> Prop :=
+  | dom_fst : `{InDom ((a,b)::rst) a}
+  | dom_rst : `{InDom l a -> InDom ((a',b')::l) a}.
 
 Inductive MapsTo {A B} : list (A * B) -> A -> B -> Prop :=
   | map_fst : `{MapsTo ((a,b)::rst) a b}
@@ -124,8 +137,8 @@ Qed.
 
 Definition in_aval := In.
 
-Definition in_list_list {A B} (l : list (A * (list B))) (a : A) (b : B) : Prop :=
-  exists bs, In (a,bs) l /\ In b bs.
+Definition in_list_list {A B} (l : list (A * (set B))) (a : A) (b : B) : Prop :=
+  exists bs, In (a,bs) l /\ set_In b bs.
 
 Inductive in_force (σ : Store) : forall (v v' : val), Prop :=
 | forced : `{in_force σ v v}
@@ -162,35 +175,83 @@ Proof.
              |auto]
    |injection H; intros; subst; constructor
    |constructor; [|apply IH];auto].
-Qed. 
+Qed.
 Definition lookup_ρ := lookup_map name_eq_dec (B := Addr).
 Definition lookup_σ := lookup_map addr_eq_dec (B := AbsVal).
-
-Fixpoint list_add_nodup {A} (eq_dec : dec_type A) (l : list A) (a : A) : list A :=
-  match l with
-      nil => a::nil
-    | a'::l' => if eq_dec a a' then l else a'::(list_add_nodup eq_dec l' a)
-  end.
-Fixpoint list_append_nodup {A} (eq_dec : dec_type A) (l l' : list A) :=
-  match l with
-      nil => l'
-    | a::l => list_add_nodup eq_dec (list_append_nodup eq_dec l l') a
-  end.
 
 Fixpoint list_join {A B C}
          (eq_dec : dec_type A)
          (combine : list (A * B) -> B -> C -> B)
          (base : list (A * B) -> C -> B)
-         (l : list (A * B))
          (l_orig : list (A * B))
-         (a : A) (c : C) : list (A * B) :=
-  (fix inner l :=
+         (a : A) (c : C)
+         (l : list (A * B)) : list (A * B) :=
   match l with
       | nil => (a,base l_orig c)::nil
       | (a',b)::l' => if (eq_dec a a') then
                         (a,(combine l_orig b c))::l'
-                       else (a',b)::(inner l')
-  end) l.
+                      else (a',b)::(list_join eq_dec combine base l_orig a c l')
+  end.
+
+Lemma in_list_join :
+  forall A B (combine : list (A * set B) -> set B -> B -> set B) base l l' a c
+    (eq_dec : dec_type A),
+    (forall l b c, set_In c (combine l b c)) ->
+    (forall l c, set_In c (base l c)) ->
+    (forall ab, In ab l -> In ab l') ->
+  in_list_list (list_join eq_dec combine base l' a c l) a c.
+Proof.
+  intros A B combine base l l' a c eq_dec Hextensive Hsingleton Hcontain.
+  induction l; simpl.
+  exists (base l' c); split; [left| apply Hsingleton]; auto.
+  destruct a0 as [a' b]; destruct (eq_dec a a') as [Heq | Hneq];
+  [subst; exists (combine l' b c); split; [left|apply Hextensive]; auto
+  |].
+  destruct IHl as [bs [Hainbs Hbinbs]].
+   (* backchain IHl *)
+    intros (a_,bs') Hin; apply Hcontain; right; auto.
+  exists bs; split; [right|]; auto.
+Qed.
+
+Lemma in_list_join2 :
+  forall A B (combine : list (A * set B) -> set B -> B -> set B) base l l' a a' c c'
+    (eq_dec : dec_type A),
+    (forall l b c c', set_In c' b -> set_In c' (combine l b c)) ->
+    (forall l b c, set_In c (combine l b c)) ->
+    (forall l c, set_In c (base l c)) ->
+    (forall ab, In ab l -> In ab l') ->
+  in_list_list l a' c' ->
+  in_list_list (list_join eq_dec combine base l' a c l) a' c'.
+Proof.
+  intros A B combine base l l' a a' c c' eq_dec Hextensive1 Hextensive2 Hsingleton Hcontain Hold.
+  induction l; simpl;
+  inversion Hold as [bs [Hpairin Hsetin]];
+  [(* base case *) inversion Hpairin
+  |destruct a0; destruct (eq_dec a a0) as [Heq | Hneq]; subst;
+   [(* Heq *)
+     destruct (eq_dec a0 a') as [Heq' | Hneq']; subst;
+    [(* Heq' *)
+      inversion Hpairin as [Hpeq|Hrest];[
+        injection Hpeq; intros; subst;
+        exists (combine l' bs c); split; [left; auto|apply Hextensive1]
+       |exists bs; split; [right|]]; auto
+    |(* Hneq' *)
+      inversion Hpairin as [Hbad|Hrest]; [
+        injection Hbad; intros; subst; contradict Hneq'|
+        exists bs; split; [right|]]; auto]
+    |(* Hneq *)]].
+  destruct (eq_dec a0 a') as [Heq' | Hneq']; subst;
+  inversion Hpairin as [Hpeq|Hrest]; try solve
+  [ (* Heq', Hpeq *)
+    injection Hpeq; intros; subst;
+      exists bs; split; [left|]; auto
+   |(* Heq', Hrest *)
+   assert (Hneed : in_list_list l a' c') by (exists bs; split; auto);
+     assert (Hcontain' : forall ab, In ab l -> In ab l') by (intros ab Hin; apply Hcontain; right; auto);
+     destruct (IHl Hcontain' Hneed) as [bs' [H0 H1]]; exists bs'; split; [right|]; auto].
+Qed.
+
+Definition singleton {A} (eq_dec : dec_type A) (x : A) : set A := set_add eq_dec x (@empty_set A).
 
 Definition force (σ : Store) (v:val) : AbsVal :=
   match v with
@@ -199,39 +260,54 @@ Definition force (σ : Store) (v:val) : AbsVal :=
                       | Some vs => vs
                     end
       | amany vs => vs
-      | v => v::nil
+      | v => singleton val_eq_dec v
   end.
 Definition absval_join (vs vs' : AbsVal) :=
-  list_append_nodup val_eq_dec vs vs'.
+  set_union val_eq_dec vs vs'.
 
 Definition σ_join (σ : Store) (a : Addr) (v : val) : Store :=
   list_join addr_eq_dec
             (fun σ_orig vs v => (absval_join vs (force σ_orig v)))
-            force σ σ a v.
+            force σ a v σ.
 Section StandardSemantics.
 Variable alloc : CESK -> Addr.
 Variable tick : CESK -> Time.
+Variable time0 : Time.
 
 Inductive red_cesk : CESK -> CESK -> Prop :=
-  ev_var : `{let s := (ev (var x) ρ σ κ t) in
+  ev_var : `{let s := (shell (ev (var x) ρ σ) κ t) in
              MapsTo ρ x a ->
-             red_cesk s (co (adelay a) σ κ (tick s))}
-| ev_app : `{let s := (ev (app e0 e1) ρ σ κ t) in
-             red_cesk s (ev e0 ρ σ ((ar e1 ρ)::κ) (tick s))}
-| ev_lam : `{let s := (ev (lam x e) ρ σ κ t) in
-             red_cesk s (co (closure x e ρ) σ κ (tick s))}
-| co_ar : `{let s := (co v σ ((ar e ρ)::κ) t) in
-            red_cesk s (ev e ρ σ ((fn v)::κ) (tick s))}
-| co_fn : `{let s := (co v σ ((fn fnv)::κ) t) in
+             red_cesk s (shell (co (adelay a) σ) κ (tick s))}
+| ev_app : `{let s := (shell (ev (app e0 e1) ρ σ) κ t) in
+             red_cesk s (shell (ev e0 ρ σ) ((ar e1 ρ)::κ) (tick s))}
+| ev_lam : `{let s := (shell (ev (lam x e) ρ σ) κ t) in
+             red_cesk s (shell (co (closure x e ρ) σ) κ (tick s))}
+| co_ar : `{let s := (shell (co v σ) ((ar e ρ)::κ) t) in
+            red_cesk s (shell (ev e ρ σ) ((fn v)::κ) (tick s))}
+| co_fn : `{let s := (shell (co v σ) ((fn fnv)::κ) t) in
             in_force σ (closure x e ρ) fnv ->
-            red_cesk s (ap x e ρ v σ κ (tick s))}
-| do_ap : `{let s := (ap x e ρ v σ κ t) in
+            red_cesk s (shell (ap x e ρ v σ) κ (tick s))}
+| do_ap : `{let s := (shell (ap x e ρ v σ) κ t) in
             let a := alloc s in
             let ρ' := extend_ρ x a ρ in
             let σ' := σ_join σ a v in
-            red_cesk s (ev e ρ' σ' κ (tick s))}.
-End StandardSemantics.
+            red_cesk s (shell (ev e ρ' σ') κ (tick s))}.
 
+Section stream.
+  Variable A : Type.
+
+  CoInductive stream : Type :=
+  | Cons : A -> stream -> stream
+  | Nil : stream.
+End stream.
+
+CoInductive Trace {State} (s0 : State) (R : State -> State -> Prop) : stream State -> Prop :=
+  | initial : Trace s0 R (Cons s0 (Nil _))
+  | CESK_step : `{Trace s0 R (Cons ς π) ->
+                  R ς ς' ->
+                  Trace s0 R (Cons ς' (Cons ς π))}.
+
+Definition CESK_trace (e : Expr) := Trace (shell (ev e nil nil) nil time0) red_cesk.
 Section NonStandardData.
 Inductive Context :=
   context : Expr -> Env -> Store -> Context.
@@ -242,7 +318,7 @@ Defined.
 
 Inductive Result :=
   res: val -> Store -> Result.
-Definition Results := list Result.
+Definition Results := set Result.
 
 Definition result_eq_dec : dec_type Result.
   decide equality; try solve [apply val_eq_dec | apply store_eq_dec].
@@ -257,22 +333,46 @@ Definition trunkont_eq_dec : dec_type TrunKont.
   decide equality; try solve [apply frame_eq_dec | apply context_eq_dec].
 Defined.
 
-Definition TrunKonts := list TrunKont.
+Definition TrunKonts := set TrunKont.
 Definition Memo := list (Context * Results).
 Definition KTable := list (Context * TrunKonts).
 
-Definition trunckonts_join (κs κs' : TrunKonts) := list_append_nodup trunkont_eq_dec κs κs'.
+Definition memo_eq_dec : dec_type Memo.
+  decide equality;
+  decide equality; try solve [apply context_eq_dec | apply list_eq_dec, result_eq_dec].
+Defined.
+
+Definition ktable_eq_dec : dec_type KTable.
+  decide equality;
+  decide equality; try solve [apply context_eq_dec | apply list_eq_dec, trunkont_eq_dec].
+Defined.
+
+Definition trunckonts_join (κs κs' : TrunKonts) := set_union trunkont_eq_dec κs κs'.
 Definition lookup_M := lookup_map context_eq_dec (B := Results).
 Definition lookup_Ξ := lookup_map context_eq_dec (B := TrunKonts).
 
 Definition Ξ_join (Ξ : KTable) (ctx : Context) (κ : TrunKont) : KTable :=
   list_join context_eq_dec
-            (fun _ κs κ => (list_add_nodup trunkont_eq_dec κs κ))
-            (fun _ κ => κ :: nil) Ξ Ξ ctx κ.
+            (fun _ κs κ => (set_add trunkont_eq_dec κ κs))
+            (fun _ κ => singleton trunkont_eq_dec κ) Ξ ctx κ Ξ.
 Definition M_join (M : Memo) (ctx : Context) (r : Result) : Memo :=
   list_join context_eq_dec
-            (fun _ rs r => (list_add_nodup result_eq_dec rs r))
-            (fun _ r => r :: nil) M M ctx r.
+            (fun _ rs r => (set_add result_eq_dec r rs))
+            (fun _ r => singleton result_eq_dec r) M ctx r M.
+
+Fixpoint map_join {A B} (join1 : list (A * B) -> A -> B -> list (A * B)) (l l' : list (A * B)) :=
+  match l with
+      nil => l'
+    | (a,b)::l'' => join1 (map_join join1 l'' l') a b
+  end.
+Definition Ξs_join := map_join (fun Ξ ctx κs => list_join context_eq_dec
+                                                          (fun _ κs' κs => set_union trunkont_eq_dec κs' κs)
+                                                          (fun _ κs => κs)
+                                                          Ξ ctx κs Ξ).
+Definition Ms_join := map_join (fun M ctx rs => list_join context_eq_dec
+                                                          (fun _ rs' rs => set_union result_eq_dec rs' rs)
+                                                          (fun _ rs => rs)
+                                                          M ctx rs M).
 
 Definition in_ctxs (Ξ : KTable) (ctx : Context) (κ : TrunKont) : Prop :=
   in_list_list Ξ ctx κ.
@@ -280,81 +380,125 @@ Definition in_ctxs (Ξ : KTable) (ctx : Context) (κ : TrunKont) : Prop :=
 Definition in_memos (M : Memo) (ctx : Context) (r : Result) : Prop :=
   in_list_list M ctx r.
 
+Inductive WShell (P : Type) :=
+  wshell : P -> TrunKont -> Time -> WShell P.
 
-Inductive WCESKMΞ :=
-  | evmk : Expr -> Env -> Store -> TrunKont -> Time -> WCESKMΞ
-  | comk : val -> Store -> TrunKont -> Time -> WCESKMΞ
-  | apmk : Name -> Expr -> Env -> (* Closure *)
-           val -> (* Argument *)
-           Store -> TrunKont -> Time -> WCESKMΞ.
+Definition WCESKMΞ := WShell CES_point.
 
 Definition wceskmξ_eq_dec : dec_type WCESKMΞ.
-  decide equality; try solve [apply expr_eq_dec | apply store_eq_dec | apply trunkont_eq_dec | apply time_eq_dec | apply val_eq_dec | apply env_eq_dec | apply name_eq_dec].
-Defined. 
+  decide equality; try solve [apply ces_point_eq_dec | apply trunkont_eq_dec | apply time_eq_dec].
+Defined.
 Inductive CESKMΞ :=
   | widemk : WCESKMΞ -> Memo -> KTable -> CESKMΞ.
+
+Definition ceskmξ_eq_dec : dec_type CESKMΞ.
+  decide equality; try solve [apply wceskmξ_eq_dec | apply memo_eq_dec | apply ktable_eq_dec].
+Defined.
 
 Section NonStandardSemantics.
 Variable allocmk : CESKMΞ -> Addr.
 Variable tickmk : CESKMΞ -> Time.
+Variable time0mk : Time.
 
 Inductive red_ceskmk : CESKMΞ -> CESKMΞ -> Prop :=
-  evmk_var : `{let s := widemk (evmk (var x) ρ σ κ t) M Ξ in
+  evmk_var : `{let s := widemk (wshell (ev (var x) ρ σ) κ t) M Ξ in
              MapsTo ρ x a ->
-             red_ceskmk s (widemk (comk (adelay a) σ κ (tickmk s))  M Ξ)}
-| evmk_app : `{let s := widemk (evmk (app e0 e1) ρ σ κ t) M Ξ in
-             red_ceskmk s (widemk (evmk e0 ρ σ (kpush (ar e1 ρ) κ) (tickmk s)) M Ξ)}
-| evmk_lam : `{let s := widemk (evmk (lam x e) ρ σ κ t) M Ξ in
-             red_ceskmk s (widemk (comk (closure x e ρ) σ κ (tickmk s)) M Ξ)}
-| comk_ar : `{let s := widemk (comk v σ (kpush (ar e ρ) κ) t) M Ξ in
-            red_ceskmk s (widemk (evmk e ρ σ (kpush (fn v) κ) (tickmk s)) M Ξ)}
-| comk_fn : `{let s := widemk (comk v σ (kpush (fn fnv) κ) t) M Ξ in
+             red_ceskmk s (widemk (wshell (co (adelay a) σ) κ (tickmk s))  M Ξ)}
+| evmk_app : `{let s := widemk (wshell (ev (app e0 e1) ρ σ) κ t) M Ξ in
+             red_ceskmk s (widemk (wshell (ev e0 ρ σ) (kpush (ar e1 ρ) κ) (tickmk s)) M Ξ)}
+| evmk_lam : `{let s := widemk (wshell (ev (lam x e) ρ σ) κ t) M Ξ in
+             red_ceskmk s (widemk (wshell (co (closure x e ρ) σ) κ (tickmk s)) M Ξ)}
+| comk_ar : `{let s := widemk (wshell (co v σ) (kpush (ar e ρ) κ) t) M Ξ in
+            red_ceskmk s (widemk (wshell (ev e ρ σ) (kpush (fn v) κ) (tickmk s)) M Ξ)}
+| comk_fn : `{let s := widemk (wshell (co v σ) (kpush (fn fnv) κ) t) M Ξ in
               in_force σ (closure x e ρ) fnv ->
-              red_ceskmk s (widemk (apmk x e ρ v σ κ (tickmk s)) M Ξ)}
-| do_apmk : `{let s := widemk (apmk x e ρ v σ κ t) M Ξ in
+              red_ceskmk s (widemk (wshell (ap x e ρ v σ) κ (tickmk s)) M Ξ)}
+| do_apmk : `{let s := widemk (wshell (ap x e ρ v σ) κ t) M Ξ in
               let a := allocmk s in
               let ρ' := extend_ρ x a ρ in
               let σ' := σ_join σ a v in
               let ctx := (context e ρ' σ') in
               let Ξ' := Ξ_join Ξ ctx κ in
               Unmapped M ctx ->
-              red_ceskmk s (widemk (evmk e ρ' σ' (rt ctx) (tickmk s)) M Ξ')}
-| do_memo : `{let s := widemk (apmk x e ρ v σ κ t) M Ξ in
+              red_ceskmk s (widemk (wshell (ev e ρ' σ') (rt ctx) (tickmk s)) M Ξ')}
+| do_memo : `{let s := widemk (wshell (ap x e ρ v σ) κ t) M Ξ in
               let a := allocmk s in
               let ρ' := extend_ρ x a ρ in
               let σ' := σ_join σ a v in
               let ctx := (context e ρ' σ') in
               let Ξ' := Ξ_join Ξ ctx κ in
               in_memos M ctx (res vm σm) ->
-              red_ceskmk s (widemk (comk vm σm κ (tickmk s)) M Ξ')} (* XXX: tick? *)
-| do_rt : `{let s := widemk (comk v σ (rt ctx) t) M Ξ in
+              red_ceskmk s (widemk (wshell (co vm σm) κ (tickmk s)) M Ξ')} (* XXX: tick? *)
+| do_rt : `{let s := widemk (wshell (co v σ) (rt ctx) t) M Ξ in
             let M' := M_join M ctx (res v σ) in
             in_ctxs Ξ ctx κ ->
-            red_ceskmk s (widemk (comk v σ κ (tickmk s)) M' Ξ)}.
+            red_ceskmk s (widemk (wshell (co v σ) κ (tickmk s)) M' Ξ)}.
 
-Definition step_all (s : CESKMΞ) : list CESKMΞ :=
+Inductive Dom_in_Dom {A B C} : list (A * B) -> list (A * C) -> Prop :=
+  | no_dom : `{Dom_in_Dom nil l}
+  | cons_dom : `{(exists b, In (a,b) l')-> Dom_in_Dom l l' -> Dom_in_Dom ((a,b)::l) l'}.
+
+Lemma In_join : forall A B C (eq_dec: dec_type A) (l l' : list (A * B))
+                        (f : list (A * B) -> B -> C -> B)  g a a' b b',
+                  (forall a b, In (a,b) l -> In (a,b) l') ->
+                  In (a,b) l ->
+                  exists b'', In (a,b'') (list_join eq_dec f g l' a' b' l).
+Proof.
+  intros A B C eq_dec l l' f g a a' b b' Hcontain Hin; induction l as [|(a0,b0) l_ IH];
+  inversion Hin;
+  assert (IHneed : forall a b, In (a,b) l_ -> In (a,b) l') by
+      (intros; apply Hcontain; right; auto);
+  pose (rec := IH IHneed);
+  [injection H; intros; subst;
+   unfold list_join;
+   destruct (eq_dec a' a) as [Heq | Hneq];[
+     subst; exists (f l' b b')
+    |exists b]; constructor; auto
+  |unfold list_join;
+    destruct (eq_dec a' a0) as [Heq | Hneq];[
+      exists b; right; auto
+           | destruct rec as [b'' Hb'']; auto; exists b''; right; auto]].
+Qed.
+
+Lemma Dom_join : forall A B C D (eq_dec: dec_type A) (l : list (A * B)) (l' : list (A * D))
+                        (f : list (A * D) -> D -> C -> D)  g a b,
+                   Dom_in_Dom l l' -> Dom_in_Dom l (list_join eq_dec f g l' a b l').
+Proof.
+  intros A B C D eq_dec l l' f g a b Hdom; induction Hdom;
+  constructor;
+  (induction l';[destruct H as [? bad]; inversion bad |]);
+  [destruct H as [b' Hb'];
+    apply In_join with (b := b')|]; auto.
+Qed.
+
+Definition TraceTo {State} (R : State -> State -> Prop) (s0 s1 : State) : Prop :=
+  exists pi, Trace s0 R (Cons s1 pi).
+
+Definition step_all (s : CESKMΞ) : set CESKMΞ :=
   match s with
-    | widemk (evmk (var x) ρ σ κ t) M Ξ  =>
+    | widemk (wshell (ev (var x) ρ σ) κ t) M Ξ  =>
       match (lookup_ρ x ρ) with
-       | None => nil
-       | Some a => (widemk (comk (adelay a) σ κ (tickmk s)) M Ξ)::nil
+       | None => empty_set _
+       | Some a => singleton ceskmξ_eq_dec (widemk (wshell (co (adelay a) σ) κ (tickmk s)) M Ξ)
       end
-    | widemk (evmk (app e0 e1) ρ σ κ t) M Ξ =>
-      (widemk (evmk e0 ρ σ (kpush (ar e1 ρ) κ) (tickmk s)) M Ξ)::nil
-    | widemk (evmk (lam x e) ρ σ κ t) M Ξ =>
-      (widemk (comk (closure x e ρ) σ κ (tickmk s)) M Ξ)::nil
-    | widemk (comk v σ (kpush (ar e ρ) κ) t) M Ξ =>
-              (widemk (evmk e ρ σ (kpush (fn v) κ) (tickmk s)) M Ξ)::nil
-    | widemk (comk v σ (kpush (fn fnv) κ) t) M Ξ =>
+    | widemk (wshell (ev (app e0 e1) ρ σ) κ t) M Ξ =>
+      singleton ceskmξ_eq_dec (widemk (wshell (ev e0 ρ σ) (kpush (ar e1 ρ) κ) (tickmk s)) M Ξ)
+    | widemk (wshell (ev (lam x e) ρ σ) κ t) M Ξ =>
+      singleton ceskmξ_eq_dec (widemk (wshell (co (closure x e ρ) σ) κ (tickmk s)) M Ξ)
+    | widemk (wshell (co v σ) (kpush (ar e ρ) κ) t) M Ξ =>
+              singleton ceskmξ_eq_dec (widemk (wshell (ev e ρ σ) (kpush (fn v) κ) (tickmk s)) M Ξ)
+    | widemk (wshell (co v σ) (kpush (fn fnv) κ) t) M Ξ =>
       (* Append forces *)
       fold_right (fun v acc =>
                     match v with
-                        closure x e ρ => (widemk (apmk x e ρ v σ κ (tickmk s)) M Ξ)::acc
+                        closure x e ρ => set_add ceskmξ_eq_dec
+                                                 (widemk (wshell (ap x e ρ v σ) κ (tickmk s)) M Ξ)
+                                                 acc
                       | _ => acc
                  end)
-                 nil
+                 (empty_set _)
                  (force σ fnv)
-    | widemk (apmk x e ρ v σ κ t) M Ξ =>
+    | widemk (wshell (ap x e ρ v σ) κ t) M Ξ =>
       let a := allocmk s in
       let ρ' := extend_ρ x a ρ in
       let σ' := σ_join σ a v in
@@ -362,42 +506,244 @@ Definition step_all (s : CESKMΞ) : list CESKMΞ :=
       let Ξ' := Ξ_join Ξ ctx κ in
       (* both call and use memo table *)
       match (lookup_M ctx M) with
-            | None => (widemk (evmk e ρ' σ' (rt ctx) (tickmk s)) M Ξ')::nil
+            | None => singleton ceskmξ_eq_dec (widemk (wshell (ev e ρ' σ') (rt ctx) (tickmk s)) M Ξ')
             | Some rs =>
               fold_right (fun r acc =>
                             match r with
-                                res vm σm => (widemk (comk vm σm κ (tickmk s)) M Ξ')::acc
+                                res vm σm => set_add ceskmξ_eq_dec
+                                                     (widemk (wshell (co vm σm) κ (tickmk s)) M Ξ')
+                                                     acc
                             end)
-                         nil
+                         (empty_set _)
                          rs
       end
-    | widemk (comk v σ (rt ctx) t) M Ξ =>
+    | widemk (wshell (co v σ) (rt ctx) t) M Ξ =>
       let M' := M_join M ctx (res v σ) in
       match (lookup_Ξ ctx Ξ) with
-          | None => nil
+          | None => (empty_set _)
           | Some κs =>
             fold_right (fun κ acc =>
-                          (widemk (comk v σ κ (tickmk s)) M' Ξ)::acc)
-                       nil κs
-      end                 
-    | widemk (comk v σ mt t) M Ξ => nil
+                          set_add ceskmξ_eq_dec
+                                  (widemk (wshell (co v σ) κ (tickmk s)) M' Ξ)
+                                  acc)
+                       (empty_set _) κs
+      end
+    | widemk (wshell (co v σ) mt t) M Ξ => empty_set _
   end.
 
-Theorem finite_steps : forall s, exists ss : list CESKMΞ, forall s',
-                         red_ceskmk s s' <-> In s' ss.
+Inductive Wide_step :=
+  wide_step : set WCESKMΞ -> Memo -> KTable -> Wide_step.
+
+Inductive System :=
+  system : set WCESKMΞ -> set WCESKMΞ -> Memo -> KTable -> System.
+
+
+Definition smush_steps (s : WCESKMΞ) (M: Memo) (Ξ: KTable) (S : set WCESKMΞ) : Wide_step :=
+  (fix smush (ss : set CESKMΞ) (nexts : set WCESKMΞ) (M : Memo) (Ξ : KTable) :=
+     match ss with
+         nil => wide_step (filter (fun s => if In_dec wceskmξ_eq_dec s S then false else true) nexts) M Ξ
+       | (widemk s M' Ξ')::ss' => smush ss' (set_add wceskmξ_eq_dec s nexts)
+                                        (Ms_join M' M)
+                                        (Ξs_join Ξ' Ξ)
+     end)
+    (step_all (widemk s M Ξ)) nil nil nil.
+
+Theorem finite_steps : forall s, exists ss : set CESKMΞ, forall s',
+                         red_ceskmk s s' <-> set_In s' ss.
 Proof.
   intro s; exists (step_all s); intro s'; split; [intro Hred|intro Hin].
   inversion_clear Hred; simpl; try solve [left; auto|
 rewrite lookup_mapsto with (eq_dec := name_eq_dec) in H;
 unfold lookup_ρ; rewrite H; constructor; auto].
 inversion H.
-Admitted. 
+Admitted.
 
-Inductive Wide_CESKMΞ : list WCESKMΞ -> list WCESKMΞ -> Memo -> KTable ->
-                        list WCESKMΞ -> list WCESKMΞ -> Memo -> KTable -> Prop :=
-  | big_step : `{Wide_CESKMΞ (**) Seen (s::F) M Ξ (**)
-                                  (list_append_nodup wceskmξ_eq_dec F' (list_add_nodup WCESKMΞ_eq_dec Seen s))
-                                  (list_append_nodup wceskmξ_eq_dec F' F)
-                                  M' Ξ'}.
+Check smush_steps.
+
+Inductive Wide_CESKMΞ : System -> System -> Prop :=
+  | big_step : forall s M Ξ Seen F ss M' Ξ',
+                 (wide_step ss M' Ξ') = (smush_steps s M Ξ Seen) ->
+                 Wide_CESKMΞ (**) (system Seen (s::F) M Ξ) (**)
+                                  (system
+                                  (set_union wceskmξ_eq_dec ss (set_add wceskmξ_eq_dec s Seen))
+                                  (set_union wceskmξ_eq_dec F ss)
+                                  M' Ξ').
+
+Definition WCESKMΞ_trace (e : Expr) := Trace (system ((wshell (ev e nil nil) mt time0)::nil) ((wshell (ev e nil nil) mt time0)::nil) nil nil) Wide_CESKMΞ.
+
+(*
+Inductive StackUnroll_gen gen (Ξ : KTable) : Kont -> TrunKont -> set Context -> Prop :=
+  unroll_mt : forall G, StackUnroll_gen gen Ξ nil mt G
+| unroll_push : forall κ tκ (R : gen Ξ κ tκ (empty_set Context) : Prop) φ G, StackUnroll_gen gen Ξ (φ :: κ) (kpush φ tκ) G
+| unroll_rt : forall ctx G tκ κ (R : gen Ξ κ tκ (set_add context_eq_dec ctx G) : Prop),
+                ~ set_In ctx G -> in_ctxs Ξ ctx tκ ->
+                StackUnroll_gen gen Ξ κ (rt ctx) G.
+
+Check monotone3.
+Check (rel3 Kont (fun _ => TrunKont) (fun _ _ => (set Context))).
+
+
+CoInductive StackUnroll (Ξ : KTable) κ tκ G : Prop :=
+| stackunroll_fold (IN : StackUnroll_gen Ξ StackUnroll κ tκ G).
+
+*)
+
+CoInductive StackUnroll (Ξ : KTable) : Kont -> TrunKont -> list Context -> Prop :=
+  unroll_mt : forall G, StackUnroll Ξ nil mt G
+| unroll_push : forall κ tκ φ G, StackUnroll Ξ κ tκ G -> StackUnroll Ξ (φ :: κ) (kpush φ tκ) G
+| unroll_rt : forall ctx G tκ κ,
+                In ctx G ->
+                StackUnroll Ξ κ tκ (remove_one context_eq_dec ctx G) ->
+                in_ctxs Ξ ctx tκ ->
+                StackUnroll Ξ κ (rt ctx) G.
+
+Theorem unroll_with_extension : forall
+        (Ξ : KTable) (ctx : Context) (κ : Kont) (tκ tκ' : TrunKont) (G G' : list Context)
+        (hyp : StackUnroll Ξ κ tκ G) (Hsub : Sublist context_eq_dec G G'), StackUnroll (Ξ_join Ξ ctx tκ') κ tκ G'.
+Proof.
+  cofix; intros Ξ ctx κ tκ tκ' G G' hyp Hsub.
+  inversion hyp; subst;
+  [constructor
+  |apply unroll_push,unroll_with_extension with (G := G)
+  | ]; auto.
+  apply unroll_rt with (tκ := tκ0); [
+  (* In ctx0 G' *)
+  apply sublist_subset in Hsub;
+    unfold Subset in Hsub;
+    rewrite Forall_forall in Hsub;
+    apply Hsub; assumption
+  |apply unroll_with_extension with (G := (remove_one context_eq_dec ctx0 G));
+    [|apply sublist_remove];assumption
+  |(* in_ctxs*)
+    apply in_list_join2; solve [
+                             intros; apply set_add_intro1; auto
+                            | intros; apply set_add_intro2; auto 
+                            | auto]].
+Qed.
+
+Inductive KontTail : Kont -> Kont -> Prop :=
+| same_tail : `{KontTail κ κ}
+| push_tail : `{KontTail κ κ' -> KontTail κ (φ :: κ')}.
+
+Fixpoint kont_tailp (κ κ' : Kont) : bool :=
+  match (kont_eq_dec κ κ') with
+      | left eqprf => true
+      | right neqprf => match κ' with
+                            nil => false
+                          | φ :: κ' => kont_tailp κ κ'
+                        end
+  end.
+
+Lemma kont_tailp_correct : forall κ κ', kont_tailp κ κ' = true <-> KontTail κ κ'.
+Proof.
+  induction κ'; simpl;
+  [destruct (kont_eq_dec κ nil); split; intro H; subst; try solve [constructor
+                                                                  |inversion H; contradiction]
+  |destruct (kont_eq_dec κ (a :: κ')) as [Heq|Hneq]; split; intro H; subst; try solve [constructor];
+   [rewrite IHκ' in H; constructor
+   |rewrite IHκ'; inversion H; subst; [contradict Hneq|]]; auto].
+Qed.
+
+CoInductive hastail (κ : Kont) : stream CESK -> Prop :=
+  Nil_tail : hastail κ (Nil _)
+| Cons_tail : forall π p κ' t, hastail κ π -> KontTail κ κ' ->
+                           hastail κ (Cons (shell p κ' t) π).
+
+Inductive Inv : CESKMΞ -> Prop :=
+  inv : forall p κ tκ t M Ξ G,
+Dom_in_Dom M Ξ ->
+StackUnroll Ξ κ tκ G ->
+(forall e ρ σ tκ' κ' G',
+in_ctxs Ξ (context e ρ σ) tκ' ->
+StackUnroll Ξ κ' tκ' G' ->
+(exists t', TraceTo red_cesk
+                    (shell (ev e ρ σ) κ' t')
+                    (shell p κ t))
+/\
+(forall v σ'',
+   in_memos M (context e ρ σ) (res v σ'') ->
+   exists pi t' t'', (Trace (shell (ev e ρ σ) κ' t')
+                        red_cesk
+                        (Cons (shell (co v σ'') κ' t'') pi) /\
+                  hastail κ' pi))) ->
+Inv (widemk (wshell p tκ t) M Ξ).
+
+Axiom comparable_ticks : forall p κ tκ t M Ξ G,
+                           StackUnroll Ξ κ tκ G ->
+                           tick (shell p κ t) = tickmk (widemk (wshell p tκ t) M Ξ).
+
+Lemma inv_invariant : forall s s', Inv s -> red_ceskmk s s' -> Inv s'.
+Proof.
+  intros s s' Hinv Hstep.
+  inversion Hinv as [? ? ? ? ? ? G Hdom Htail Φ]; subst.
+  Ltac common Φ kont point κ t invG tightenG pushG :=
+      apply (inv (κ := kont) (G := invG)); try solve [apply unroll_push; auto
+                                                  |constructor; auto
+                                                  |auto];
+      intros e' ρ' σ' tκ' κ' G' Htκ' Hunroll;
+      pose (Φrinst := (Φ e' ρ' σ' tκ' κ' G' Htκ' Hunroll));
+      destruct Φrinst as [Φreach Φmemo];
+      destruct Φreach as [t'_ [π Φreach_path]];
+      split;[
+        (* reach *)
+        exists t'_;
+          exists (Cons (shell point κ t) π);
+          constructor; [assumption|
+                        compute;
+                          rewrite <- (comparable_ticks _ _ _ (κ := κ) (G := tightenG));
+                          solve [constructor; auto
+                                    |auto]]
+              |(* memo *) auto].
+  inversion Hstep as [? ? ? ? ? (* <- time *) ? ? ? s0 Hmap Hpeq Hs'eq |
+                      ? ? ? ? ? ? ? ? ? Hpeq |
+                      ? ? ? ? ? ? ? ? s0 Hpeq Hs'eq |
+                      ? ? ? ? ? ? ? ? s0 Hpeq Hs'eq |
+                      ? ? ? ? ? ? ? ? ? ? s0 Hin_force Hpeq Hs'eq |
+                      ? ? ? ? ? ? ? ? ? s0 a ρ' σ' ctx Ξ' Hunmapped Hpeq Hs'eq |
+                      ? ? ? ? ? ? ? ? ? ? ? s0 a ρ' σ' ctx Ξ' Hin_memos Hpeq Hs'eq |
+                      ? ? ? ? ? ? s0 M' Hin_ctxs Hpeq Hs'eq].
+  (* Var lookup *)
+  subst; common Φ κ (ev (var x) ρ σ) κ t G G G.
+  (* function eval *)
+  subst; common Φ ((ar e1 ρ)::κ) (ev (app e0 e1) ρ σ) κ t G G G.
+  (* lam *)
+  subst; common Φ κ (ev (lam x e) ρ σ) κ t G G G.
+  (* arg eval *)
+  inversion Htail as [|? ? ? ? G'' Hκtail|]; subst;
+  try discriminate;
+  injection H4; intros; subst;
+  common Φ (fn v :: κ1) (co v σ) ((ar e ρ)::κ1) t G G G''.
+  (* fn -> ap *)
+  inversion Htail as [|? ? ? ? Hκtail|]; subst;
+  try discriminate;
+  injection H4; intros; subst;
+  common Φ κ1 (co v σ) ((fn fnv)::κ1) t G G G.
+  (* do unmemoized ap *)
+  apply inv with (κ := κ) (G:= G); auto.
+  apply Dom_join; auto.
+  assert (Htail' : StackUnroll Ξ' κ tκ (ctx :: G)).
+  apply unroll_with_extension with (G := G);[assumption|].
+  apply sublist_extension with (l'' := [ ctx ]).
+ with (G' := (set_add context_eq_dec ctx G)); try solve [auto | apply subset_refl].
+  apply unroll_rt with (tκ := tκ); try solve [intro bad; inversion bad].
+  unfold in_ctxs.
+  apply in_list_join; auto;
+  intros; apply set_add_intro2; auto.
+  pose (Φrinst := (Φ e ρ' σ' (rt ctx) κ' Htκ' Htail));
+    destruct Φrinst as [Φreach Φmemo];
+    destruct Φreach as [t'_ [π Φreach_path]].
+
+Inductive state_rel : CESK -> System -> Prop :=
+  point_rel : `{StackUnroll Ξ κ κ' nil ->
+                (set_In (wshell p κ' t) Seen \/ set_In (wshell p κ' t) F) ->
+                state_rel (shell p κ t) (system Seen F M Ξ)}.
+
+Theorem simulation : forall e s, CESK_trace e π -> exists s', state_rel s s' /\ WCESKMΞ_trace e π'.
+Proof.
+  intros e s π.
+
+
 End NonStandardSemantics.
 End NonStandardData.
+End StandardSemantics.
+End Data.
